theories/NatMap.v
@@ -1,0 +1,40 @@
+From Stdlib Require Import Utf8.
+From Stdlib Require Import Structures.OrderedType.
+From Stdlib Require Import FSets.FMaps.
+From Stdlib Require Import Lia.
+
+Module NatOrdered <: OrderedType.
+  Definition t : Type := nat.
+
+  Definition eq (x: t) (y: t) := x = y.
+  Definition lt (x: t) (y: t) := x < y.
+
+  Definition eq_refl := @eq_refl t.
+  Definition eq_sym := @eq_sym t.
+  Definition eq_trans := @eq_trans t.
+
+  Definition lt_trans : ∀ x y z : t, lt x y -> lt y z -> lt x z.
+  Proof. unfold lt. lia. Qed.
+
+  Definition lt_not_eq : ∀ x y : t, lt x y -> ~ eq x y.
+  Proof. unfold eq, lt. lia. Qed.
+
+  Definition compare : ∀ x y : t, Compare lt eq x y.
+  Proof.
+    intros x y. unfold eq, lt.
+    destruct (PeanoNat.Nat.compare x y) eqn:H.
+    - apply EQ. now apply PeanoNat.Nat.compare_eq_iff.
+    - apply LT. now apply PeanoNat.Nat.compare_lt_iff.
+    - apply GT. now apply PeanoNat.Nat.compare_gt_iff.
+  Defined.
+
+  Definition eq_dec : ∀ x y, { eq x y } + { ~ eq x y }.
+  Proof.
+    intros x y. destruct (compare x y).
+    - right. now apply lt_not_eq.
+    - now left.
+    - right. symmetry. now apply lt_not_eq.
+  Defined.
+End NatOrdered.
+
+Module NatMap <: S := FMapList.Make NatOrdered.
