theories/Tactics.v
@@ -1,0 +1,11 @@
+Ltac inv H := inversion H; subst; clear H.
+
+Ltac pc_inj :=
+  match goal with
+  | [ H1: ?f = Some (?x1 ?x2), H2: ?f = Some (?y1 ?y2) |- _ ] =>
+      let H := fresh in
+      assert (H: y1 y2 = x1 x2) by congruence; inv H; clear H2
+  | [ H1: ?f = Some ?x, H2: ?f = Some ?y |- _ ] =>
+      let H := fresh in
+      assert (H: y = x) by congruence; subst; clear H2
+  end.
