theories/WP.v
@@ -1,0 +1,231 @@
+From Stdlib Require Import Utf8.
+
+From Stdlib Require Import Lists.List.
+From Stdlib Require Import Strings.String.
+From Stdlib Require Import ZArith.ZArith.
+From Stdlib Require Import Lia.
+From Stdlib Require Import Relations.Relations.
+
+From RSL Require Import NatMap.
+From RSL Require Import RTL.
+From RSL Require Import Notations.
+From RSL Require Import Semantics.
+From RSL Require Import Tactics.
+
+Import RTLNotations.
+Import ListNotations.
+
+(* Set Mangle Names. *)
+
+Section WP.
+  Variable P : program.
+
+  Definition postcondition : Type := val -> memory -> Prop.
+
+  Inductive final (Q: postcondition) : state -> Prop :=
+  | Final : ∀ v m, Q v m -> final Q ([], ReturnState v, m).
+
+  Definition safe (Q: postcondition) (s: state) : Prop :=
+    ∀ t, P ⊢ s ->>* t -> final Q t ∨ ∃ u, P ⊢ t ->> u.
+
+  Definition wp (f: function) (pc: node) (Q: postcondition)
+    : regmap * memory -> Prop :=
+    fun '(ρ, m) => safe Q ([], State f pc ρ, m).
+
+  Lemma wp_ret f pc Q : forall v,
+    f@pc is <{ ret v }> ->
+    ∀ ρ m, Q (get_reg ρ v) m -> wp f pc Q (ρ, m).
+  Proof.
+    intros v H ρ m.
+    unfold wp, safe.
+    intros Hwp t Hred.
+    destruct (inv_step _ _ _ Hred) as [ <- | (ss & Hreds & Hrtc )].
+    - right. eexists. econstructor; now eauto.
+    - inv Hreds; try congruence.
+      destruct (inv_step _ _ _ Hrtc) as [ <- | (? & Hwhat & ? )].
+      + pc_inj. left. constructor. assumption.
+      + inversion Hwhat.
+  Qed.
+
+  Lemma wp_nop f pc Q : forall pc',
+    f@pc is <{ nop -> pc' }> ->
+    ∀ ρ m, wp f pc' Q (ρ, m) -> wp f pc Q (ρ, m).
+  Proof.
+    intros pc' H ρ m.
+    unfold wp, safe.
+    intros Hwp t Hred.
+    destruct (inv_step _ _ _ Hred) as [ <- | (ss & Hreds & Hrtc )].
+    - right. eexists. econstructor; now eauto.
+    - apply Hwp; inv Hreds; pc_inj; congruence.
+  Qed.
+
+  Lemma wp_op f pc Q : forall dst op args pc',
+    f@pc is <{ dst := @op args -> pc' }> ->
+    ∀ ρ m,
+    (∃ v,
+        eval_op op (get_regs ρ args) = Some v
+        ∧ wp f pc' Q (set_reg ρ dst v, m)
+    ) -> wp f pc Q (ρ, m).
+  Proof.
+    intros dst op args pc' H ρ m.
+    unfold wp, safe.
+    intros (v & Hv & Hwp) t Hred.
+    destruct (inv_step _ _ _ Hred) as [ <- | (ss & Hreds & Hrtc )].
+    - right. eexists. econstructor; now eauto.
+    - apply Hwp; inv Hreds; pc_inj; congruence.
+  Qed.
+
+  Lemma wp_load f pc Q : forall dst src pc',
+    f@pc is <{ dst := !src -> pc' }> ->
+    ∀ ρ m,
+    (
+      let addr := get_reg ρ src in
+      ∃ v, get_at m addr = Some v ∧  wp f pc' Q (set_reg ρ dst v, m)
+    ) -> wp f pc Q (ρ, m).
+  Proof.
+    intros dst src pc' H ρ m.
+    unfold wp, safe.
+    intros (v & Hv & Hwp) t Hred.
+    destruct (inv_step _ _ _ Hred) as [ <- | (ss & Hreds & Hrtc )].
+    - right. eexists. econstructor; now eauto.
+    - apply Hwp; inv Hreds; pc_inj; try congruence.
+  Qed.
+
+  Lemma wp_store f pc Q : forall dst src pc',
+    f@pc is <{ !dst := src -> pc' }> ->
+    ∀ ρ m,
+    (
+      let addr := get_reg ρ dst in
+      let v := get_reg ρ src in
+      ∃ m', set_at m addr v = Some m' ∧ wp f pc' Q (ρ, m')
+    ) -> wp f pc Q (ρ, m).
+  Proof.
+    intros dst src pc' H ρ m.
+    unfold wp, safe.
+    intros (v & Hv & Hwp) t Hred.
+    destruct (inv_step _ _ _ Hred) as [ <- | (ss & Hreds & Hrtc )].
+    - right. eexists. econstructor; now eauto.
+    - apply Hwp; inv Hreds; pc_inj; congruence.
+  Qed.
+
+  Lemma wp_cond f pc Q : forall cond ifso ifnot,
+    f@pc is <{ if cond then goto ifso else goto ifnot }> ->
+    ∀ ρ m,
+    (
+      if (get_reg ρ cond =? 0)%Z
+      then wp f ifso Q (ρ, m)
+      else wp f ifnot Q (ρ, m)
+    ) -> wp f pc Q (ρ, m).
+  Proof.
+    intros cond ifso ifnot H ρ m.
+    unfold wp, safe.
+    intros Hwp t Hred.
+    destruct (inv_step _ _ _ Hred) as [ <- | (ss & Hreds & Hrtc)].
+    - right. eexists. econstructor; now eauto.
+    - inv Hreds; pc_inj; try congruence.
+      destruct (get_reg ρ cond =? 0)%Z eqn:Hcond; auto.
+  Qed.
+
+  Definition precondition : Type := list val -> memory -> Prop.
+
+  Definition hoare (P: precondition) (f: function) (Q: postcondition) : Prop
+    := ∀ args m, P args m -> safe Q ([], CallState f args, m).
+
+  Notation "'{{' P '}}' f '{{' Q '}}'" :=
+    (hoare P f Q) (at level 90, f at next level).
+
+  Lemma wp_call f pc Q : ∀ dst sig args pc',
+    f@pc is <{ dst := @call sig args -> pc' }> ->
+    ∀ ρ m,
+    (∃ fn Pre Post,
+        let vals := get_regs ρ args in
+        find_fun P sig = Some fn ∧
+        {{ Pre }} fn {{ Post }} ∧
+        Pre vals m ∧
+        ∀ v m', let ρ' := set_reg ρ dst v in
+                Post v m' -> wp f pc' Q (ρ', m')
+    ) -> wp f pc Q (ρ, m).
+  Proof.
+    intros dst sig args pc' H ρ m.
+    unfold wp, safe.
+    intros (fn & Pre & Post & Hfun & Hspec & Hpre & Hwp) t Hred.
+    destruct (inv_step _ _ _ Hred) as [ <- | (ss & Hreds & Hrtc)].
+    - right. eexists. econstructor; now eauto.
+    - inv Hreds; pc_inj; try congruence. pc_inj.
+      destruct t as [[σ' s] m''] eqn:Ht.
+      destruct (unfold_call _ _ _ _ _ _ _ _ _ _  _ Hrtc)
+        as [(σ'' & Hσ & Hrtc') | (v & m' & Hrtc' & Hrest)].
+      + destruct (Hspec _ _ Hpre _ Hrtc') as [Hfin | (u & Hu)].
+        * inv Hfin; simpl. right. eexists. econstructor; now eauto.
+        * right. destruct u as [[]?]. subst.
+          eexists. apply lift_step. apply Hu.
+      + destruct (Hspec _ _ Hpre _ Hrtc') as [Hfin | (u & Hu)].
+        * inv Hfin; simpl. eapply Hwp; eassumption.
+        * inversion Hu.
+  Qed.
+End WP.
+
+Section WP2.
+  Variable P : program.
+  (* Definition stuck s := ~ (∃ t, P ⊢ s ->> t) ∧ ~ (final s). *)
+
+  (* Definition not_stuck s := final s ∨ ∃ t, P ⊢ s ->> t. *)
+
+  Fixpoint wp2_ (n: nat) (s: state) (Q: postcondition) :=
+    match n with
+    | O => True
+    | S n =>
+        (final Q s) ∨ ((∃ t, P ⊢ s ->> t) ∧ ∀ t, P ⊢ s ->> t -> wp2_ n t Q)
+    end.
+
+  Definition wp2 (s: state) (Q: postcondition) := ∀ n, wp2_ n s Q.
+
+  Lemma safe_to_wp2 : ∀ s Q,
+    safe P Q s -> wp2 s Q.
+  Proof.
+    intros s Q H n. induction n as [ | n IH] in H, s |- *.
+    - easy.
+    - simpl. destruct (H s (rt_refl _ _ _)) as [Hfin | [t Ht]].
+      + auto.
+      + right. split.
+        * exists t. assumption.
+        * intros u Hu. apply IH. intros v Hv. apply H.
+          eapply rt_trans.
+          -- constructor. eassumption.
+          -- assumption.
+  Qed.
+
+  Lemma wp2_acc : ∀ s t Q,
+    P ⊢ s ->>* t ->
+    wp2 s Q ->
+    wp2 t Q.
+  Proof.
+    intros s t Q Hst.
+    induction Hst as [ s t H | s | s t u Hs IHs Ht IHt]; intros Hw.
+    - intros n. specialize (Hw (S n)). simpl in Hw.
+      destruct Hw as [Hfin | [_ Hall]].
+      + inversion Hfin; subst. inversion H.
+      + apply Hall. exact H.
+    - exact Hw.
+    - apply IHt. apply IHs. exact Hw.
+  Qed.
+
+  Lemma wp2_to_safe : ∀ s Q,
+    wp2 s Q -> safe P Q s.
+  Proof.
+    intros s Q Hwp. unfold wp2, safe.
+    intros t Hred.
+    apply (wp2_acc _ _ Q) in Hred; try assumption.
+    specialize (Hred 1). simpl in Hred.
+    destruct Hred as [?| [ ]]; auto.
+  Qed.
+
+  Theorem wp2_is_safe :
+    ∀ s Q, wp2 s Q <-> safe P Q s.
+  Proof.
+    intros s Q. split.
+    - apply wp2_to_safe.
+    - apply safe_to_wp2.
+  Qed.
+End WP2.
+
