theories/WPGenerator.v
@@ -1,0 +1,149 @@
+From Stdlib Require Import Utf8.
+From Stdlib Require Import Lists.List.
+From Stdlib Require Import Strings.String.
+From Stdlib Require Import ZArith.ZArith.
+From Stdlib Require Import Lia.
+From Stdlib Require Import Relations.Relations.
+
+From RSL Require Import NatMap.
+From RSL Require Import RTL.
+From RSL Require Import Notations.
+From RSL Require Import Semantics.
+From RSL Require Import Tactics.
+From RSL Require Import WP.
+
+Import RTLNotations.
+Import ListNotations.
+
+Section WPNaive.
+  Variable P: program.
+
+  Fixpoint wp_ (fuel: nat) (f: function) (pc: node) (Q: postcondition)
+    : regmap * memory -> Prop :=
+    match fuel with
+    | O => fun '(ρ, m) => False
+    | S n =>
+        match NatMap.find pc f.(fn_code) with
+        | Some <{ nop -> pc }> =>
+            wp_ n f pc Q
+
+        | Some <{ dst := @ op args -> pc }> =>
+            fun '(ρ, m) =>
+              ∃ v,
+                eval_op op (get_regs ρ args) = Some v ∧
+                wp_ n f pc Q (set_reg ρ dst v, m)
+
+        | Some <{ dst := ! src -> pc }> =>
+            fun '(ρ, m) =>
+              let addr := get_reg ρ src in
+              ∃ v, get_at m addr = Some v ∧
+                   wp_ n f pc Q (set_reg ρ dst v, m)
+
+        | Some <{ ! dst := src -> pc }> =>
+            fun '(ρ, m) =>
+              let addr := get_reg ρ dst in
+              let v := get_reg ρ src in
+              ∃ m', set_at m addr v = Some m' ∧
+                    wp_ n f pc Q (ρ, m')
+
+        | Some <{ if cond then goto pc1 else goto pc2 }> =>
+            fun '(ρ, m) =>
+              if (get_reg ρ cond =? 0)%Z
+              then wp_ n f pc1 Q (ρ, m)
+              else wp_ n f pc2 Q (ρ, m)
+
+        | Some <{ ret r }> =>
+            fun '(ρ, m) => Q (get_reg ρ r) m
+
+        | Some <{ dst := @call sig args -> pc }> =>
+            fun '(ρ, m) =>
+              ∃ fn Pre Post,
+                let vals := get_regs ρ args in
+                find_fun P sig = Some fn ∧
+                hoare P Pre fn Post ∧
+                Pre vals m ∧
+                ∀ v m', let ρ' := set_reg ρ dst v in
+                        Post v m' -> wp_ n f pc Q (ρ', m')
+        | None =>
+            fun σ => False
+        end
+    end.
+
+  Lemma wp_sound: ∀ fuel f pc Q ρ m,
+    wp_ fuel f pc Q (ρ, m) -> wp P f pc Q (ρ, m).
+  Proof.
+    induction fuel as [ | n IH ].
+    - easy.
+    - simpl. intros f pc Q σ H Hwp.
+      destruct (NatMap.find pc (fn_code f)) as [[] | ] eqn:Hi.
+      + eapply wp_nop; eauto.
+      + eapply wp_op; eauto.
+        destruct Hwp as (v & Hv & Hwp); eauto.
+      + eapply wp_load; eauto.
+        destruct Hwp as (v & Hv & Hwp); eauto.
+      + eapply wp_store; eauto.
+        destruct Hwp as (m' & Hm' & Hwp); eauto.
+      + eapply wp_call; eauto.
+        destruct Hwp as (fn & Pre & Post & Hfun & Hspec & Hpre & Hwp).
+        exists fn. exists Pre. exists Post. repeat split; eauto.
+      + eapply wp_cond; eauto.
+        destruct (get_reg σ r =? 0)%Z; auto.
+      + eapply wp_ret. apply Hi. auto.
+      + contradiction.
+  Qed.
+End WPNaive.
+
+Section WPGenerator.
+  Variable P : program.
+
+  Definition node_inv : Type := node -> regmap * memory -> Prop.
+
+  Record inv_sound (f : function) (I : node_inv) (Q : postcondition) : Prop :=
+  {
+    sound_ret : ∀ pc v,
+      f@pc is <{ ret v }> ->
+      ∀ ρ m, I pc (ρ, m) -> Q (get_reg ρ v) m
+
+  ; sound_nop : ∀ pc pc',
+      f@pc is <{ nop -> pc' }> ->
+      ∀ ρ m, I pc (ρ, m) -> I pc' (ρ, m)
+
+  ; sound_op : ∀ pc dst op args pc',
+      f@pc is <{ dst := @op args -> pc' }> ->
+      ∀ ρ m, I pc (ρ, m) ->
+             ∃ v,
+               eval_op op (get_regs ρ args) = Some v
+               ∧ I pc' (set_reg ρ dst v, m)
+
+  ; sound_load : ∀ pc dst src pc',
+      f@pc is <{ dst := !src -> pc' }> ->
+      ∀ ρ m, I pc (ρ, m) ->
+             ∃ v,
+               get_at m (get_reg ρ src) = Some v
+               ∧ I pc' (set_reg ρ dst v, m)
+
+  ; sound_store : ∀ pc dst src pc',
+      f@pc is <{ !dst := src -> pc' }> ->
+      ∀ ρ m, I pc (ρ, m) ->
+             ∃ m',
+               set_at m (get_reg ρ dst) (get_reg ρ src) = Some m'
+               ∧ I pc' (ρ, m')
+
+  ; sound_cond : ∀ pc cond ifso ifnot,
+      f@pc is <{ if cond then goto ifso else goto ifnot }> ->
+      ∀ ρ m, I pc (ρ, m) ->
+             if (get_reg ρ cond =? 0)%Z
+             then I ifso (ρ, m)
+             else I ifnot (ρ, m)
+
+  ; sound_call : ∀ pc dst sig args pc',
+      f@pc is <{ dst := @call sig args -> pc' }> ->
+      ∀ ρ m, I pc (ρ, m) ->
+             ∃ fn Pre Post,
+               find_fun P sig = Some fn
+               ∧ hoare P Pre fn Post
+               ∧ Pre (get_regs ρ args) m
+               ∧ ∀ v m', Post v m' -> I pc' (set_reg ρ dst v, m')
+  }.
+
+End WPGenerator.
